verify mutexguard_deref_shr

theories/typing/lib/mutex/mutexguard.v
@@ -28,28 +28,30 @@ Section mutexguard.
       __poison: poison::Guard,
     }
   *)
+  Context `{!BiFUpd PROP}.
+Implicit Type P Q R: PROP.
 
   Program Definition mutexguard {𝔄} (κ: lft) (ty: type 𝔄) : type (predₛ 𝔄) := {|
     ty_size := 1;  ty_lfts := κ :: ty.(ty_lfts);  ty_E := ty.(ty_E) ++ ty_outlives_E ty κ;
+    (* One logical step is required for [ty_share] *)
     ty_own Φπ d tid vl := ⌜d > 0⌝ ∗ [loc[l] := vl] ∃Φ κ',
       ⌜Φπ = const Φ⌝ ∗ κ ⊑ κ' ∗ κ' ⊑ ty.(ty_lft) ∗
       &at{κ, mutexN} (lock_proto l (mutex_body ty Φ κ' l tid)) ∗
       mutex_body ty Φ κ' l tid;
-    ty_shr Φπ _ κ' tid l := ∃Φ (l': loc) κᵢ,
-      ⌜Φπ = const Φ⌝ ∗ κ ⊓ κ' ⊑ κᵢ ∗ κᵢ ⊑ ty.(ty_lft) ∗
-      &frac{κ'}(λ q', l ↦{q'} #l') ∗
-      □ ∀E q, ⌜↑lftN ∪ ↑shrN ⊆ E⌝ -∗ q.[κᵢ] ={E,E∖↑shrN}=∗▷|={E∖↑shrN}=>
-        ∃(vπ: proph 𝔄) d, ⟨π, Φ (vπ π)⟩ ∗ ⧖(S d) ∗
-          |={E∖↑shrN}=>|={E∖↑shrN}▷=>^d |={E∖↑shrN,E}=>
-            ty.(ty_shr) vπ d κᵢ tid (l' +ₗ 1) ∗ q.[κᵢ];
+    ty_shr Φπ _ κ' tid l := ∃Φ (l': loc) κᵢ (vπ: proph 𝔄) d,
+      ⌜Φπ = const Φ⌝ ∗ κ' ⊑ κᵢ ∗ κᵢ ⊑ ty.(ty_lft) ∗
+      &frac{κ'}(λ q', l ↦{q'} #l') ∗ ⟨π, Φ (vπ π)⟩ ∗ ⧖(S d) ∗
+      □ ∀E q, ⌜↑lftN ∪ ↑shrN ⊆ E⌝ -∗ q.[κᵢ]
+        ={E,E∖↑shrN}=∗ |={E∖↑shrN}▷=>^(S d) |={E∖↑shrN,E}=>
+          ty.(ty_shr) vπ d κᵢ tid (l' +ₗ 1) ∗ q.[κᵢ];
   |}%I.
   Next Obligation. iIntros (??????[|[[]|][]]) "[%?] //". Qed.
   Next Obligation. iIntros "*% [%$] !%". lia. Qed.
   Next Obligation. done. Qed.
   Next Obligation.
-    iIntros "* #Inκ' (%&%&%&->& ⊑κᵢ & κᵢ⊑ & Bor & inv)". iExists _, _, _.
-    iFrame "κᵢ⊑ inv". iSplit; [done|]. iSplit; [|by iApply frac_bor_shorten].
-    iApply lft_incl_trans; [|done]. iApply lft_intersect_mono; by [iApply lft_incl_refl|].
+    iIntros "%%* #Inκ' (%&%&%&%&%&->& ⊑κᵢ & κᵢ⊑ & Bor & big)".
+    iExists _, _, _, _, _. iFrame "κᵢ⊑ big". iSplit; [done|].
+    iSplit; [|by iApply frac_bor_shorten]. by iApply lft_incl_trans.
   Qed.
   Next Obligation.
     iIntros (????? d κ') "*% #LFT #In Bor κ' //".
@@ -67,26 +69,26 @@ Section mutexguard.
     iMod (bor_sep with "LFT Bor") as "[_ Bor]"; [done|].
     iMod (bor_unnest with "LFT Bor") as "Bor"; [done|]. iIntros "/=!>!>!>!>".
     iApply step_fupdN_full_intro. iMod "Bor". set κᵢ := κ'' ⊓ κ'.
-    iMod (inv_alloc shrN _ (_ ∨ ∃(vπ: proph 𝔄) d, ⟨π, Φ (vπ π)⟩ ∗ ⧖(S d) ∗
-      ty.(ty_shr) vπ d κᵢ tid (l' +ₗ 1))%I with "[Bor]") as "#inv".
+    iAssert (κ' ⊑ κᵢ)%I as "κ'⊑κᵢ".
+    { iApply lft_incl_glb; [|iApply lft_incl_refl]. iApply lft_incl_trans; [|done].
+      iApply lft_incl_trans; [done|]. iApply lft_intersect_incl_l. }
+    iMod (lft_incl_acc with "κ'⊑κᵢ κ'") as (?) "[κᵢ Toκ']"; [done|].
+    do 2 (iMod (bor_exists_tok with "LFT Bor κᵢ") as (?) "[Bor κᵢ]"; [done|]).
+    iMod (bor_sep_persistent with "LFT Bor κᵢ") as "(>Obs & Bor & κᵢ)"; [done|].
+    iMod (bor_sep_persistent with "LFT Bor κᵢ") as "(>⧖ & Bor & κᵢ)"; [done|].
+    iMod ("Toκ'" with "κᵢ") as "κ'".
+    iMod (inv_alloc shrN _ (_ ∨ ty.(ty_shr) _ _ _ _ _)%I with "[Bor]") as "#inv".
     { iLeft. iNext. iExact "Bor". }
-    iModIntro. iFrame "κ'". iExists _, _, κᵢ. iSplit; [done|]. iFrame "Bor↦".
-    iSplit. { iApply lft_intersect_mono; [done|iApply lft_incl_refl]. }
-    iAssert (κᵢ ⊑ ty.(ty_lft))%I as "#?".
+    iModIntro. iFrame "κ'". iExists _, _, κᵢ, _, _. iSplit; [done|].
+    iFrame "Bor↦ Obs ⧖ κ'⊑κᵢ". iAssert (κᵢ ⊑ ty.(ty_lft))%I as "#?".
     { iApply lft_incl_trans; [iApply lft_intersect_incl_l|done]. }
     iSplit; [done|]. iIntros "!>" (???) "κᵢ".
-    iInv shrN as "[Bor|big]" "Close"; iIntros "!>!>"; last first.
-    { iDestruct "big" as (??) "(#Obs & #⧖ & #ty)". iModIntro. iExists _, _.
-      iFrame "κᵢ Obs ⧖". iApply step_fupdN_full_intro. iModIntro.
-      iMod ("Close" with "[]"); [|done]. iNext. iRight. iExists _, _.
-      iFrame "Obs ⧖ ty". }
-    do 2 (iMod (bor_exists_tok with "LFT Bor κᵢ") as (?) "[Bor κᵢ]"; [solve_ndisj|]).
-    iMod (bor_sep_persistent with "LFT Bor κᵢ") as "(>#Obs & Bor & κᵢ)"; [solve_ndisj|].
-    iMod (bor_sep_persistent with "LFT Bor κᵢ") as "(>#⧖ & Bor & κᵢ)"; [solve_ndisj|].
-    iModIntro. iExists _, _. iFrame "Obs ⧖".
+    iInv shrN as "[Bor|#ty]" "Close"; iIntros "/=!>!>!>"; last first.
+    { iApply step_fupdN_full_intro. iModIntro. iFrame "κᵢ".
+      iMod ("Close" with "[]"); by [iRight|]. }
     iMod (ty_share with "LFT [] Bor κᵢ") as "Upd"; [solve_ndisj|done|].
     iApply (step_fupdN_wand with "Upd"). iIntros "!> >[#ty $]".
-    iMod ("Close" with "[]"); [|done]. iNext. iRight. iExists _, _. iFrame "Obs ⧖ ty".
+    iMod ("Close" with "[]"); by [iRight|].
   Qed.
   Next Obligation.
     iIntros (???????[|[[]|][]]) "*% _ _ [% big] //". iDestruct "big" as (??->) "?".
@@ -94,9 +96,9 @@ Section mutexguard.
     do 2 (iSplit; [done|]). iIntros "_!>". iSplit; [done|]. iExists _, _. by iFrame.
   Qed.
   Next Obligation.
-    iIntros "*% _ _ _ (%&%&%&->& big) $ !>!>!>". iApply step_fupdN_full_intro.
+    iIntros "*% _ _ _ (%&%&%&%&%&->&?) $ !>!>!>". iApply step_fupdN_full_intro.
     iModIntro. iExists [], 1%Qp. do 2 (iSplit; [done|]). iIntros "_!>".
-    iExists _, _, _. by iFrame.
+    iExists _, _, _, _, _. by iFrame.
   Qed.
 
   Global Instance mutexguard_ne {𝔄} κ : NonExpansive (mutexguard (𝔄:=𝔄) κ).
@@ -109,8 +111,8 @@ Section mutexguard.
     - move=>/= *. do 10 f_equiv. { by apply equiv_dist, lft_incl_equiv_proper_r. }
       rewrite /mutex_body.
       f_equiv; [do 2 f_equiv|]; f_contractive; do 9 f_equiv; by simpl in *.
-    - move=>/= *. do 9 f_equiv. { by apply equiv_dist, lft_incl_equiv_proper_r. }
-      do 21 (f_contractive || f_equiv). by simpl in *.
+    - move=>/= *. do 13 f_equiv. { by apply equiv_dist, lft_incl_equiv_proper_r. }
+      do 17 (f_contractive || f_equiv). by simpl in *.
   Qed.
 
   Global Instance mutexguard_sync {𝔄} κ (ty: type 𝔄) :
@@ -138,8 +140,8 @@ Section mutexguard.
     - iIntros (????? vl) "*% _ _ $ (%& big) !>". case vl as [|[[]|][]]=>//.
       iDestruct "big" as (??->) "?". iApply step_fupdN_full_intro. iModIntro.
       iSplit; [by iExists _|]. iSplit; [done|]. iExists _, _. by iFrame.
-    - iIntros "*% _ _ $ (%&%&%&->&?) !>!>!>". iApply step_fupdN_full_intro.
-      iModIntro. iSplit; [by iExists _|]. iExists _, _, _. by iFrame.
+    - iIntros "*% _ _ $ (%&%&%&%&%&->&?) !>!>!>". iApply step_fupdN_full_intro.
+      iModIntro. iSplit; [by iExists _|]. iExists _, _, _, _, _. by iFrame.
   Qed.
 
   Lemma mutexguard_subtype {𝔄 𝔅} κ κ' f g `{!@Iso 𝔄 𝔅 f g} ty ty' E L :
@@ -157,15 +159,12 @@ Section mutexguard.
       iDestruct (mutex_body_iff with "InOwn") as "Iff". iSplit; [|by iApply "Iff"].
       iApply at_bor_shorten; [done|]. iApply (at_bor_iff with "[] At"). iNext.
       by iApply lock_proto_iff_proper.
-    - iIntros "* (%&%& %κᵢ &->&#?&#?&#?& #big)". iExists _, _, κᵢ.
-      iSplit; [done|]. iSplit.
-      { iApply lft_incl_trans; [|done].
-        iApply lft_intersect_mono; [done|iApply lft_incl_refl]. }
-      iSplit. { by iApply lft_incl_trans. } iSplit; [done|]. iIntros "!>%%% κᵢ".
-      iMod ("big" with "[//] κᵢ") as "big'". iIntros "!>!>".
-      iMod "big'" as (??) "(Obs & ⧖ & Upd)". iModIntro. iExists (f ∘ _), _.
-      iFrame "⧖". iSplit. { iApply proph_obs_eq; [|done]=>/= ?. by rewrite semi_iso'. }
-      iApply (step_fupdN_wand with "Upd"). iIntros ">[ty $] !>". by iApply "InShr".
+    - iIntros "* (%&%& %κᵢ &%&%&->&#?&#?&#?&#?&#?& #big)".
+      iExists _, _, κᵢ, (f ∘ _), _. do 2 (iSplit; [done|]).
+      iSplit; [by iApply lft_incl_trans|]. iSplit; [done|].
+      iSplit. { iApply proph_obs_eq; [|done]=>/= ?. by rewrite semi_iso'. }
+      iSplit; [done|]. iIntros "!>" (???) "κᵢ". iMod ("big" with "[//] κᵢ") as "Upd".
+      iApply (step_fupdN_wand with "Upd"). iIntros "!> >[?$] !>". by iApply "InShr".
   Qed.
   Lemma mutexguard_eqtype {𝔄 𝔅} κ κ' f g `{!@Iso 𝔄 𝔅 f g} ty ty' E L :
     lctx_lft_eq E L κ' κ → eqtype E L ty ty' f g →
@@ -225,14 +224,15 @@ Section mutexguard.
     iApply type_delete; [solve_typing..|].
     iApply type_jump; solve_typing.
   Qed.
+*)
 
-  Definition mutexguard_derefmut : val :=
+  Definition mutexguard_deref: val :=
     fn: ["g"] :=
-      let: "g'" := !"g" in
-      let: "m" := !"g'" in
+      let: "g'" := !"g" in let: "m" := !"g'" in
       letalloc: "r" <- ("m" +ₗ #1) in
       delete [ #1; "g"];; return: ["r"].
 
+(*
   Lemma mutexguard_derefmut_type ty :
     typed_val mutexguard_derefmut
               (fn(∀ '(α, β), ∅; &uniq{α}(mutexguard β ty)) → &uniq{α}ty).
@@ -277,46 +277,47 @@ Section mutexguard.
     iApply type_delete; [solve_typing..|].
     iApply type_jump; solve_typing.
   Qed.
+*)
 
-  Definition mutexguard_deref : val := mutexguard_derefmut.
-
-  Lemma mutexguard_deref_type ty :
-    typed_val mutexguard_derefmut
-              (fn(∀ '(α, β), ∅; &shr{α}(mutexguard β ty)) → &shr{α}ty).
+  Lemma mutexguard_deref_shr_type {𝔄} (ty: type 𝔄) :
+    typed_val mutexguard_deref
+      (fn<(α, β)>(∅; &shr{α} (mutexguard β ty)) → &shr{α} ty)
+      (λ post '-[Φ], ∀a: 𝔄, Φ a → post a).
   Proof.
-    intros E L. iApply type_fn; [solve_typing..|]. iIntros "/= !>".
-      iIntros ([α β] ϝ ret arg). inv_vec arg=>g. simpl_subst.
-    iApply type_deref; [solve_typing..|]; iIntros (g'); simpl_subst.
-    (* Switch to Iris. *)
-    iIntros (tid) "#LFT #HE Hna HL Hk [Hg [Hg' _]]".
-    rewrite !tctx_hasty_val [[g]]lock /=.
-    destruct g' as [[|lg|]|]; try done. simpl.
-    iDestruct "Hg'" as (lm) "[Hlg Hshr]".
-    iMod (lctx_lft_alive_tok α with "HE HL") as (qα) "([Hα1 Hα2] & HL & Hclose1)";
+    eapply type_fn; [solve_typing|]=>/= αβ ??[g[]]. case αβ=> α β. simpl_subst.
+    iIntros (?[?[]]?) "LFT #TIME _ _ #E Na L C /=[g _] Obs". rewrite tctx_hasty_val.
+    iDestruct "g" as ([|d]) "[_ box]"=>//. case g as [[|g|]|]=>//.
+    iDestruct "box" as "[(%vl & >↦g & guard) †g]".
+    case d as [|]; try by iDestruct "guard" as ">[]".
+    case vl as [|[[|l|]|][]]; try by iDestruct "guard" as ">[]".
+    rewrite heap_mapsto_vec_singleton. wp_read. wp_let.
+    iDestruct "guard" as (?????->) "(#⊑κᵢ &?& Bor↦ & Obs' & #⧖ & #Upd)".
+    iCombine "Obs Obs'" as "#?".
+    iMod (lctx_lft_alive_tok α with "E L") as (?) "(α & L & ToL)";
       [solve_typing..|].
-    iMod (frac_bor_acc with "LFT Hlg Hα1") as (qlx') "[H↦ Hclose2]"; first done.
-    iMod (lctx_lft_alive_tok β with "HE HL") as (qβ) "(Hβ & HL & Hclose3)";
-      [solve_typing..|].
-    iDestruct (lft_intersect_acc with "Hβ Hα2") as (qβα) "[Hα2β Hclose4]".
-    wp_bind (!_)%E. iApply (wp_step_fupd with "[Hshr Hα2β]");
-         [|by iApply ("Hshr" with "[] Hα2β")|]; first done.
-    wp_read. iIntros "[#Hshr Hα2β] !>". wp_let.
-    iDestruct ("Hclose4" with "Hα2β") as "[Hβ Hα2]".
-    iMod ("Hclose3" with "Hβ HL") as "HL".
-    iMod ("Hclose2" with "H↦") as "Hα1".
-    iMod ("Hclose1" with "[$] HL") as "HL".
-    iDestruct (lctx_lft_incl_incl α β with "HL HE") as "#Hαβ"; [solve_typing..|].
-    (* Switch back to typing mode. *)
-    iApply (type_type _ _ _ [ g ◁ own_ptr _ _; #lm +ₗ #1 ◁ &shr{α} ty ]
-        with "[] LFT HE Hna HL Hk"); last first.
-    { rewrite tctx_interp_cons tctx_interp_singleton tctx_hasty_val tctx_hasty_val' //.
-      unlock. iFrame. iApply ty_shr_mono; last done.
-      iApply lft_incl_glb; last by iApply lft_incl_refl. done. }
-    iApply type_letalloc_1; [solve_typing..|]; iIntros (r); simpl_subst.
-    iApply type_delete; [solve_typing..|].
-    iApply type_jump; solve_typing.
+    iMod (frac_bor_acc with "LFT Bor↦ α") as (?) "[>↦l Toα]"; [done|].
+    wp_read. wp_let. iMod ("Toα" with "↦l") as "α".
+    iMod (lft_incl_acc with "⊑κᵢ α") as (?) "[κᵢ Toα]"; [done|].
+    wp_bind (new _). iSpecialize ("Upd" $! ⊤ with "[//] κᵢ").
+    iApply (wp_step_fupdN_persistent_time_receipt _ _ ∅ with "TIME ⧖ [Upd]");
+      [done|done| |].
+    { iApply step_fupdN_with_emp. rewrite difference_empty_L.
+      iApply (step_fupdN_nmono (S _)); [|done]. lia. }
+    iApply wp_new; [done..|]. iIntros "!>% [†r ↦r] [ty κᵢ] !>". wp_let.
+    iMod ("Toα" with "κᵢ") as "α". iMod ("ToL" with "α L") as "L".
+    rewrite heap_mapsto_vec_singleton. wp_op. wp_write. wp_bind (delete _).
+    rewrite -heap_mapsto_vec_singleton freeable_sz_full.
+    iApply (wp_persistent_time_receipt with "TIME ⧖"); [done|]. iClear "⧖".
+    iApply (wp_delete with "[$↦g $†g]"); [done|]. iIntros "!>_ #⧖".
+    do 3 wp_seq. rewrite cctx_interp_singleton.
+    iApply ("C" $! [# #_] -[_] with "Na L [-] []"); last first.
+    { iApply proph_obs_impl; [|done]=>/= ?[Imp ?]. by apply Imp. }
+    rewrite/= right_id (tctx_hasty_val #_). iExists _. iSplit; [done|].
+    rewrite/= freeable_sz_full. iFrame "†r". iNext. iExists [_].
+    rewrite heap_mapsto_vec_singleton. iFrame "↦r". by iApply ty_shr_lft_mono.
   Qed.
 
+(*
   Definition mutexguard_drop : val :=
     fn: ["g"] :=
       let: "m" := !"g" in
